isabelle - further work on statement typechecking soundness, including an improved definition of sound_statement_result

isabelle/core/CoreTyEnv.thy
@@ -34,6 +34,9 @@ record CoreTyEnv =
   (* Type variable bindings: for polymorphic contexts *)
   TE_TypeVars :: "string fset"
 
+  (* Expected return type of the enclosing function *)
+  TE_ReturnType :: CoreType
+
   (* Function signatures *)
   TE_Functions :: "(string, FunInfo) fmap"
 
@@ -53,5 +56,30 @@ record CoreTyEnv =
      sizes are not known. A datatype is ghost if any of its constructor payloads
      contains MathInt, MathReal, or another ghost datatype. *)
   TE_GhostDatatypes :: "string fset"
+
+(* tyenv_subset env1 env2: env1 is a "sub-environment" of env2.
+   This means env2 has all the same variables (with the same types) plus possibly more.
+   The "fixed" fields (functions, datatypes, return type, type vars) must be identical. *)
+definition tyenv_subset :: "CoreTyEnv \<Rightarrow> CoreTyEnv \<Rightarrow> bool" where
+  "tyenv_subset env1 env2 \<equiv>
+    (\<forall>name ty. fmlookup (TE_TermVars env1) name = Some ty \<longrightarrow>
+               fmlookup (TE_TermVars env2) name = Some ty) \<and>
+    TE_GhostVars env1 |\<subseteq>| TE_GhostVars env2 \<and>
+    TE_ConstNames env1 |\<subseteq>| TE_ConstNames env2 \<and>
+    TE_ReturnType env1 = TE_ReturnType env2 \<and>
+    TE_Functions env1 = TE_Functions env2 \<and>
+    TE_Datatypes env1 = TE_Datatypes env2 \<and>
+    TE_DataCtors env1 = TE_DataCtors env2 \<and>
+    TE_DataCtorsByType env1 = TE_DataCtorsByType env2 \<and>
+    TE_GhostDatatypes env1 = TE_GhostDatatypes env2 \<and>
+    TE_TypeVars env1 = TE_TypeVars env2"
+
+lemma tyenv_subset_refl: "tyenv_subset env env"
+  unfolding tyenv_subset_def by simp
+
+lemma tyenv_subset_trans:
+  assumes "tyenv_subset env1 env2" and "tyenv_subset env2 env3"
+  shows "tyenv_subset env1 env3"
+  using assms unfolding tyenv_subset_def by (auto dest: fsubset_trans)
 
 end
